add Inductive Prop

Lambda.v
@@ -11,11 +11,6 @@ Inductive type : Set :=
     BoolT : type
   | FunT  : type -> type -> type.
 
-Definition type_dec : forall t1 t2 : type, {t1 = t2} + {t1 <> t2}.
-Proof.
-  decide equality.
-Qed.
-
 Inductive term : Set :=
     Var     : string -> term
   | Bool    : bool   -> term
@@ -23,7 +18,28 @@ Inductive term : Set :=
   | Apply   : term  -> term -> term
   | If      : term -> term -> term -> term.
 
-(* Eval *)
+(* equality *)
+Definition type_dec : forall t1 t2 : type, {t1 = t2} + {t1 <> t2}.
+Proof.
+  decide equality.
+Qed.
+
+(* Prop *)
+Inductive Value  : term -> Prop :=
+  | ValVar    : forall s : string, Value (Var s)
+  | ValBool   : forall b : bool,   Value (Bool b)
+  | ValLambda : forall (x : string) (ty : type) (body : term), Value (Lambda x ty body).
+
+Inductive Reducible : term -> Prop :=
+  | RAppLeft  : forall t1 t2 : term, Reducible t1 -> Reducible (Apply t1 t2)
+  | RAppRight : forall t1 t2 : term, Reducible t2 -> Reducible (Apply t1 t2)
+  | RLambda   : forall (x : string) (ty : type) (body arg : term), Reducible (Apply (Lambda x ty body) arg)
+  | RIfCond   : forall (t1 t2 t3 : term), Reducible t1 -> Reducible (If t1 t2 t3)
+  | RIf       : forall (b : bool) (t1 t2 : term), Reducible (If (Bool b) t1 t2).
+
+Definition tenv := list (string * type).
+
+(* function *)
 Fixpoint subst (t : term) (old : string) (new : term) :=
   match t with
     | Bool _ =>
@@ -52,15 +68,15 @@ Definition is_value (t : term) :=
       false
   end.
 
-Fixpoint eval (t : term) :=
+Fixpoint reduce (t : term) :=
   match t with
     Var _   | Bool _  | Lambda _ _ _ =>
       None
   | Apply t1 t2 =>
-      match eval t1 with
+      match reduce t1 with
         Some t => Some (Apply t t2)
       | None =>
-      	 match eval t2 with
+      	 match reduce t2 with
 	  Some t => Some (Apply t1 t)
        	| None   =>
       	   match t1 with
@@ -74,7 +90,7 @@ Fixpoint eval (t : term) :=
   | If (Bool false) t2 t3 =>
       Some t3
   | If t1 t2 t3 =>
-      match eval t1 with
+      match reduce t1 with
       	None   => None
       | Some t => Some (If t t2 t3)
       end
@@ -92,7 +108,7 @@ Fixpoint assoc {A : Type} (x : string) (xs : list (string * A)) :=
       	assoc x ys
   end.
 
-Fixpoint typing (t : term) (tenv : list (string * type)) :=
+Fixpoint typing (t : term) (tenv : tenv) :=
   match t with
     Bool _ =>
       Some BoolT
@@ -129,7 +145,104 @@ Fixpoint typing (t : term) (tenv : list (string * type)) :=
     end
   end.
 
-(* theorem *)
+(* prop theorem *)
+Theorem value_prop :
+  forall t : term, is_value t = true <-> Value t.
+Proof.
+split.
+ destruct t.
+  intro; apply ValVar.
+
+  intro; apply ValBool.
+
+  intro; apply ValLambda.
+
+  simpl in |- *; intro; discriminate.
+
+  simpl in |- *; intro; discriminate.
+
+ generalize t.
+ apply Value_ind.
+  intro; reflexivity.
+
+  intro; reflexivity.
+
+  intro; reflexivity.
+Qed.
+
+(*Theorem reduce_prop :
+  forall t r : term, Some r = reduce t <-> Reducible t.
+split.
+ generalize r.
+ induction t.
+  simpl in |- *; intros; discriminate.
+
+  simpl in |- *; intros; discriminate.
+
+  simpl in |- *; intros; discriminate.
+
+  intro.
+  simpl in |- *.
+  destruct (reduce t1).
+   intros.
+   apply RAppLeft.
+   eapply IHt1.
+   reflexivity.
+
+   destruct (reduce t2).
+    intros.
+    apply RAppRight.
+    eapply IHt2.
+    reflexivity.
+
+    destruct t1.
+     intro; discriminate.
+
+     intro; discriminate.
+
+     intro.
+     apply RLambda.
+
+     intro; discriminate.
+
+     intro; discriminate.
+
+  intro; simpl in |- *.
+  destruct t1.
+   simpl in |- *.
+   intro; discriminate.
+
+   intro.
+   apply RIf.
+
+   simpl in |- *; intro; discriminate.
+
+   destruct (reduce (Apply t1_1 t1_2)).
+    intro.
+    apply RIfCond.
+    eapply IHt1.
+    reflexivity.
+
+    intro; discriminate.
+
+   destruct (reduce (If t1_1 t1_2 t1_3)).
+    intro.
+    apply RIfCond.
+    eapply IHt1.
+    reflexivity.
+
+    intro; discriminate.
+
+ generalize t.
+ apply Reducible_ind.
+  <Your Tactic Text here>
+  <Your Tactic Text here>
+  <Your Tactic Text here>
+  <Your Tactic Text here>
+  <Your Tactic Text here>
+Error: Attempt to save an incomplete proof
+*)
+
 Definition value (t : term) :=
   match t with
     Var _   | Bool _  | Lambda _ _ _ =>
